model/agp32RelationScript.sml
@@ -28,7 +28,7 @@ End
 Definition isMemOp_isa_op_def:
   isMemOp_isa_op nop a =
   if nop = NONE then F
-  else isMemOp_isa (FUNPOW Next (THE nop - 1) a)
+  else isMEM_stg_op_isa (FUNPOW Next (THE nop - 1) a)
 End
 
 Definition reg_adr_update_isa_def:
@@ -45,7 +45,7 @@ Definition enable_stg_def:
   else if k = 2 then s.ID.ID_ID_write_enable
   else if k = 3 then s.ID.ID_EX_write_enable
   else if k = 4 then s.MEM.MEM_state_flag \/ s.MEM.MEM_enable
-  else if k = 5 then (s.MEM.MEM_write_enable /\ s.WB.WB_state_flag) \/ s.WB.WB_enable
+  else if k = 5 then s.WB.WB_state_flag \/ s.WB.WB_enable
   else F
 End
 
@@ -114,7 +114,6 @@ Definition Init_def:
   ~s.MEM.MEM_state_flag /\
   ~s.MEM.MEM_enable /\
   ~s.MEM.MEM_write_reg /\
-  ~s.MEM.MEM_write_enable /\
   ~s.WB.WB_enable /\
   ~s.WB.WB_write_reg
 End
