model/compilation/agp32VerilogScript.sml
@@ -14,7 +14,7 @@ local
               "acc_arg", "acc_arg_ready", "acc_res", "acc_res_ready", "interrupt_req",
               "PC", "ID_PC", "EX_PC", "EX_imm", "EX_addrW", "EX_opc",
               "MEM_PC", "MEM_dataA", "MEM_dataB", "MEM_ALU_res",
-              "MEM_SHIFT_res", "MEM_write_enable", "MEM_addrW", "MEM_opc",
+              "MEM_SHIFT_res", "MEM_addrW", "MEM_opc",
               "WB_write_reg", "WB_addrW", "MEM_enable", "WB_enable"]
 in
  val tstate = init_translator module_def
